good

Phi_System/Phi_BI.thy
@@ -1643,21 +1643,35 @@ ML_file \<open>library/tools/simproc_ExSet_expand_quantifier.ML\<close>
 
 subsubsection \<open>ToA Reasoning\<close>
 
-lemma [\<phi>reason %ToA_fixes_quant]:
+lemma skolemize_transformation[\<phi>reason %ToA_fixes_quant]:
   "(\<And>x.  T x \<t>\<r>\<a>\<n>\<s>\<f>\<o>\<r>\<m>\<s> U \<w>\<i>\<t>\<h> P x)
 \<Longrightarrow> ExSet T \<t>\<r>\<a>\<n>\<s>\<f>\<o>\<r>\<m>\<s> U \<w>\<i>\<t>\<h> Ex P"
   unfolding Transformation_def by simp fastforce
 
-lemma [\<phi>reason %ToA_fixes_quant+5]:
+lemma skolemize_transformation_R[\<phi>reason %ToA_fixes_quant+5]:
   "(\<And>x.  T x \<t>\<r>\<a>\<n>\<s>\<f>\<o>\<r>\<m>\<s> U \<r>\<e>\<m>\<a>\<i>\<n>\<s>[C] R x \<w>\<i>\<t>\<h> P x)
 \<Longrightarrow> ExSet T \<t>\<r>\<a>\<n>\<s>\<f>\<o>\<r>\<m>\<s> U \<r>\<e>\<m>\<a>\<i>\<n>\<s>[C] ExSet R \<w>\<i>\<t>\<h> Ex P"
   unfolding Transformation_def REMAINS_def by (cases C; simp; blast)
 
-lemma aaax[\<phi>reason %ToA_fixes_quant+5]:
+lemma skolemize_transformation_tR[\<phi>reason %ToA_fixes_quant+5]:
   "(\<And>x.  T x \<t>\<r>\<a>\<n>\<s>\<f>\<o>\<r>\<m>\<s> \<phi>TagA mode (U \<r>\<e>\<m>\<a>\<i>\<n>\<s>[C] R x) \<w>\<i>\<t>\<h> P x)
 \<Longrightarrow> ExSet T \<t>\<r>\<a>\<n>\<s>\<f>\<o>\<r>\<m>\<s> \<phi>TagA mode (U \<r>\<e>\<m>\<a>\<i>\<n>\<s>[C] ExSet R) \<w>\<i>\<t>\<h> Ex P"
   unfolding Transformation_def REMAINS_def \<phi>TagA_def
   by (cases C; simp; blast)
+
+ML \<open>
+fun skolemize_transformation th =
+ (case Phi_Syntax.dest_transformation (Thm.major_prem_of th)
+    of (Const(\<^const_name>\<open>ExSet\<close>, _) $ _,
+        Const(\<^const_name>\<open>\<phi>TagA\<close>, _) $ _ $ (Const(\<^const_name>\<open>REMAINS\<close>, _) $ _ $ _ $ _), _) =>
+        skolemize_transformation (@{thm' skolemize_transformation_tR} RS th)
+     | (Const(\<^const_name>\<open>ExSet\<close>, _) $ _,
+        Const(\<^const_name>\<open>REMAINS\<close>, _) $ _ $ _ $ _, _) =>
+        skolemize_transformation (@{thm' skolemize_transformation_R} RS th)
+     | (Const(\<^const_name>\<open>ExSet\<close>, _) $ _, _, _) =>
+        skolemize_transformation (@{thm' skolemize_transformation} RS th)
+     | _ => th)
+\<close>
 
 lemma [\<phi>reason %ToA_fixes_quant]:
   "(\<And>x. T x * W \<t>\<r>\<a>\<n>\<s>\<f>\<o>\<r>\<m>\<s> U \<w>\<i>\<t>\<h> P x)
@@ -4889,7 +4903,7 @@ fun conv_transformation_by_assertion_ss ctxt =
                                      (Simplifier.rewrite target_ctxt)
                                      Conv.all_conv
   end
-
+(*
 fun skolemization_transformation C ctxt =
   let fun skolem ctxt ctm =
         case Phi_Syntax.dest_transformation (Thm.term_of ctm)
@@ -4900,6 +4914,7 @@ fun skolemization_transformation C ctxt =
    in conv_transformation_by_assertion_ss ctxt then_conv
       skolem ctxt
   end
+*)
 \<close>
 
 thm BI_Skolem[folded atomize_eq, THEN Meson.TruepropI, folded atomize_all]
@@ -5887,11 +5902,14 @@ fn (_, (ctxt0,sequent)) => Seq.make (fn () =>
               Conv.combination_conv (Conv.arg_conv (insert_tag_src ctxt)) (insert_tag_src ctxt) ctm
            | _ => Conv.rewr_conv rule ctm*)
 
-      val sequent = Conv.gconv_rule (Phi_Conv.hhf_concl_conv (
-            skolemization_transformation (fn ctxt =>
-              Phi_Syntax.transformation_conv (insert_tag_src ctxt) (insert_tag_tgt ctxt) Conv.all_conv)
+      val sequent = Conv.gconv_rule (Phi_Conv.hhf_concl_conv (fn ctxt =>
+            conv_transformation_by_assertion_ss ctxt
           ) ctxt) 1 sequent
-
+      val sequent = skolemize_transformation sequent
+      val sequent = Conv.gconv_rule (Phi_Conv.hhf_concl_conv (fn ctxt =>
+            Phi_Syntax.transformation_conv (insert_tag_src ctxt) (insert_tag_tgt ctxt) Conv.all_conv
+          ) ctxt) 1 sequent
+(*ExSet_transformation*)
       val sequent = @{thm "_NToA_init_"} RS sequent
 
       val ctxt = Config.restore under_NToA_ctxt ctxt0 ctxt
